Work in progress on bridging lemma for composition theorem.

common/UCComposition.ec
@@ -2,7 +2,7 @@
 
 require import UCCore UCListAux.
 
-abstract theory CompRF.
+abstract theory CompBridge.
 
 (* begin theory parameters *)
 
@@ -73,7 +73,7 @@ module MakeRFComp (Rest : FUNC, Par : FUNC) : FUNC = {
         }
         elif (addr_ge_param rf_info self m.`3.`1) {
           pari <- head_of_drop_size_first 0 self m.`3.`1;
-          if (! (nth1_adv_pi_begin_params rf_info pari < m.`2.`2 <=
+          if (! (nth1_adv_pi_begin_params rf_info pari <= m.`2.`2 <=
                  nth1_adv_pi_end_params rf_info pari)) {
             r <- None;
           }
@@ -115,4 +115,172 @@ module MakeRFComp (Rest : FUNC, Par : FUNC) : FUNC = {
   }
 }.
 
-end CompRF.
+clone MakeInterface as MakeInt'
+proof *.
+
+module MI' = MakeInt.MI.
+
+module CompEnv (Rest : FUNC, Env : ENV, Inter : INTER) = {
+  var stub_st : msg option
+  var func : addr
+  var in_guard_low : int fset
+
+  module StubPar : FUNC = {
+    proc init(func : addr) : unit = { }
+
+    proc invoke(m : msg) : msg option = {
+      var r : msg option;
+      if (stub_st <> None) {
+        r <- stub_st; stub_st <- None;
+      }
+      else {
+        r <@ Inter.invoke(m);
+        if (r <> None) {
+          m <- oget r;
+          if (m.`1 = Adv) {
+            stub_st <- Some m;
+            (* only mode and destination port matter (destination port id
+               must not be 0) *)
+            r <-
+              Some
+              (Adv, (adv, 1), (func ++ [change_pari], 1), TagNoInter, []);
+          }
+        }
+      }
+      return r;
+    }
+  }
+
+  module StubAdv : ADV = {
+    proc init() : unit = { }
+
+    proc invoke(m : msg) : msg option = {
+      var r : msg option;
+      if (stub_st <> None) {
+        r <- stub_st; stub_st <- None;
+      }
+      else {
+        r <@ Inter.invoke(m);
+        if (r <> None) {
+          m <- oget r;
+          if (m.`1 = Dir) {
+            stub_st <- Some m;
+            (* only mode and destination address matter *)
+            r <-
+              Some
+              (Adv, (func ++ [change_pari], 1), (adv, 1), TagNoInter, []);
+          }
+        }
+      }
+      return r;
+    }
+  }
+
+  (* func_ will end with change_pari *)
+
+  proc main(func_ : addr, in_guard : int fset) : bool = {
+    var b : bool;
+    stub_st <- None;
+    func <- take (size func_ - 1) func_;
+    b <@ Exper(MI'(MakeRFComp(Rest, StubPar), StubAdv), Env)
+           .main(func, in_guard_low);
+    return b;
+  }
+}.
+
+op rest_adv_pi_ok (guard : int fset) : bool =
+  (forall (advpi : int),
+   rf_info.`rfi_adv_pi_begin < advpi <= rf_info.`rfi_adv_pi_main_end =>
+   advpi \in guard) /\
+  (forall (advpi pari : int),
+   (1 <= pari < change_pari \/
+    change_pari < pari <= rf_info.`rfi_num_params) =>
+   (nth1_adv_pi_begin_params rf_info pari <= advpi <=
+    nth1_adv_pi_end_params rf_info pari) =>
+   advpi \in guard).
+
+section.
+
+declare module Env  <: ENV.
+declare module Adv  <: ADV{-Env}.
+declare module Rest <: FUNC{-Env, -Adv}.
+declare module Par  <: FUNC{-Env, -Adv, -Rest}.
+
+declare op term_rest : glob Rest -> int.
+declare op term_par  : glob Par -> int.
+
+declare axiom ge0_term_rest (gl : glob Rest) :
+  0 <= term_rest gl.
+
+declare axiom rest_down (n : int) :
+   equiv
+   [Rest.invoke ~ Rest.invoke :
+    ={m, glob Rest} /\ term_rest (glob Rest){1} = n ==>
+    ={res, glob Rest} /\
+    (res{1} = None \/ term_rest (glob Rest){1} < n)].
+
+declare axiom ge0_term_par (gl : glob Par) :
+  0 <= term_par gl.
+
+declare axiom par_down (n : int) :
+   equiv
+   [Par.invoke ~ Par.invoke :
+    ={m, glob Par} /\ term_par (glob Par){1} = n ==>
+    ={res, glob Par} /\
+    (res{1} = None \/ term_par (glob Par){1} < n)].
+
+lemma comp_bridge
+      (func' : addr, in_guard_low' in_guard_hi' : int fset) &m :
+  in_guard_low' \subset in_guard_hi' => rest_adv_pi_ok in_guard_hi' =>
+  CompEnv.in_guard_low{m} = in_guard_low' =>
+  Pr[Exper(MI(MakeRFComp(Rest, Par), Adv), Env)
+       .main(func', in_guard_low') @ &m : res] =
+  Pr[Exper(MI(Par, Adv), CompEnv(Rest, Env))
+       .main(func' ++ [change_pari], in_guard_hi') @ &m : res].
+proof.
+admit.
+qed.
+
+end section.
+
+print comp_bridge.
+
+lemma compos_bridge
+      (Env <: ENV) (Adv <: ADV{-Env})
+      (Rest <: FUNC{-Env, -Adv})
+      (Par <: FUNC{-Env, -Adv, -Rest})
+      (term_rest : glob Rest -> int, term_par : glob Par -> int)
+      (func' : addr, in_guard_low' in_guard_hi' : int fset) &m :
+  (forall (gl : glob Rest), 0 <= term_rest gl) =>
+  (forall (n : int),
+   equiv
+   [Rest.invoke ~ Rest.invoke :
+    ={m, glob Rest} /\ term_rest (glob Rest){1} = n ==>
+    ={res, glob Rest} /\
+    (res{1} = None \/ term_rest (glob Rest){1} < n)]) =>
+  (forall (gl : glob Par), 0 <= term_par gl) =>
+  (forall (n : int),
+   equiv
+   [Par.invoke ~ Par.invoke :
+    ={m, glob Par} /\ term_par (glob Par){1} = n ==>
+    ={res, glob Par} /\
+    (res{1} = None \/ term_par (glob Par){1} < n)]) =>
+  in_guard_low' \subset in_guard_hi' => rest_adv_pi_ok in_guard_hi' =>
+  CompEnv.in_guard_low{m} = in_guard_low' =>
+  Pr[Exper(MI(MakeRFComp(Rest, Par), Adv), Env)
+       .main(func', in_guard_low') @ &m : res] =
+  Pr[Exper(MI(Par, Adv), CompEnv(Rest, Env))
+       .main(func' ++ [change_pari], in_guard_hi') @ &m : res].
+proof.
+move => ge0_term_rest term_rest_down ge0_term_par term_par_down.
+move => H1 H2 H3.
+apply
+  (comp_bridge Env Adv Rest Par
+   term_rest term_par
+   ge0_term_rest term_rest_down
+   ge0_term_par term_par_down
+   _ _ _ &m) => //.
+qed.
+
+end CompBridge.
+
